src/reify_gen.ml
@@ -1,7 +1,5 @@
-let resolve_symbol (contrib_name : string) (path : string list) (tm : string) : Term.constr =
-  let re = Coqlib.find_reference contrib_name path tm in
-  Libnames.constr_of_global re
-
+(** Module types for monads **)
+(*****************************)
 module type MONAD =
 sig
   type 'a m
@@ -28,6 +26,8 @@ sig
   val local : (env -> env) -> 'a m -> 'a m
 end
 
+(** Module types for reification **)
+(**********************************)
 module type REIFY =
 sig
   type result
@@ -46,6 +46,9 @@ sig
                   Term.constr -> Term.constr array -> result m
 end
 
+(** Reification Instances **)
+(***************************)
+
 module ReifyMap (R : REIFY)
 		(F : sig type result
 			 val map : R.result R.m -> result R.m
@@ -59,14 +62,14 @@ struct
   let reify t = F.map (R.reify t)
 end
 
-(** The simplest instantiation is just an environment of
- ** expressions. This can be used for both expressions and types
+(** Reification based on environments of terms.
  **)
-module ReifyEnv (M : MONAD)
-                (S : STATE with type state = Term.constr list
-                           with type 'a m = 'a M.m)
-	      : REIFY with type 'a m = 'a M.m
-		      with type result = int =
+module ReifyEnv
+  (M : MONAD)
+  (S : STATE with type state = Term.constr option list
+             with type 'a m = 'a M.m)
+  : REIFY with type 'a m = 'a M.m
+          with type result = int =
 struct
   type result = int
   type 'a m = 'a M.m
@@ -75,14 +78,16 @@ struct
     let rec env_get i x =
       match x with
 	[] -> None
-      | x :: xs ->
+      | Some x :: xs ->
 	if Term.eq_constr x k
 	then Some i
 	else env_get (i+1) xs
+      | None :: xs ->
+	env_get (i+1) xs
     in env_get 0
 
   let env_app a b =
-    (List.append a [b], List.length a)
+    (List.append a [Some b], List.length a)
 
   let reify (t : Term.constr) : int m =
     M.bind S.get (fun e ->
@@ -106,93 +111,120 @@ let as_arrow t =
   with
     Invalid_argument _ -> None
 
-let to_positive contrib =
-  let pos_pkg = ["Coq";"Numbers";"BinNums"] in
-  let xH = lazy (resolve_symbol contrib pos_pkg "xH") in
-  let xO = lazy (resolve_symbol contrib pos_pkg "xO") in
-  let xI = lazy (resolve_symbol contrib pos_pkg "xI") in
-  let rec to_positive n =
-    if n = 1 then
-      Lazy.force xH
-    else
-      if n mod 2 = 0 then
-	Term.mkApp (Lazy.force xO, [| to_positive (n / 2) |])
+module Std (C : sig val contrib_name : string end) =
+struct
+  let resolve_symbol (path : string list) (tm : string) : Term.constr =
+    let re = Coqlib.find_reference C.contrib_name path tm in
+    Libnames.constr_of_global re
+
+  let datatypes_pkg = ["Coq";"Init";"Datatypes"]
+  let none = lazy (resolve_symbol datatypes_pkg "None")
+  let some = lazy (resolve_symbol datatypes_pkg "Some")
+
+  let to_option typ (x : Term.constr option) =
+    match x with
+      None -> Term.mkApp (Lazy.force none, [| typ |])
+    | Some x -> Term.mkApp (Lazy.force some, [| typ ; x |])
+
+  let to_positive =
+    let pos_pkg = ["Coq";"Numbers";"BinNums"] in
+    let xH = lazy (resolve_symbol pos_pkg "xH") in
+    let xO = lazy (resolve_symbol pos_pkg "xO") in
+    let xI = lazy (resolve_symbol pos_pkg "xI") in
+    let rec to_positive n =
+      if n = 1 then
+	Lazy.force xH
       else
-  	Term.mkApp (Lazy.force xI, [| to_positive (n / 2) |])
-  in
-  fun n ->
-    if n <= 0
-    then raise (Invalid_argument ("to_positive: " ^ string_of_int n))
-    else to_positive n
+	if n mod 2 = 0 then
+	  Term.mkApp (Lazy.force xO, [| to_positive (n / 2) |])
+	else
+  	  Term.mkApp (Lazy.force xI, [| to_positive (n / 2) |])
+    in
+    fun n ->
+      if n <= 0
+      then raise (Invalid_argument ("to_positive: " ^ string_of_int n))
+      else to_positive n
 
-let to_N contrib =
-  let n_pkg = ["Coq";"Numbers";"BinNums"] in
-  let o = lazy (resolve_symbol contrib n_pkg "N0") in
-  let pos = lazy (resolve_symbol contrib n_pkg "Npos") in
-  let to_pos = to_positive contrib in
-  fun n ->
-    if n = 0
-    then Lazy.force o
-    else
+  let to_N =
+    let n_pkg = ["Coq";"Numbers";"BinNums"] in
+    let o = lazy (resolve_symbol n_pkg "N0") in
+    let pos = lazy (resolve_symbol n_pkg "Npos") in
+    fun n ->
+      if n = 0
+      then Lazy.force o
+      else
+	if n < 0
+	then raise (Invalid_argument ("to_N: " ^ string_of_int n))
+	else Term.mkApp (Lazy.force pos, [| to_positive n |])
+
+  let to_nat =
+    let s = lazy (resolve_symbol datatypes_pkg "S") in
+    let o = lazy (resolve_symbol datatypes_pkg "O") in
+    let rec to_nat n =
+      if n = 0 then
+	Lazy.force o
+      else
+	Term.mkApp (Lazy.force s, [| to_nat (n - 1) |])
+    in
+    fun n ->
       if n < 0
-      then raise (Invalid_argument ("to_N: " ^ string_of_int n))
-      else Term.mkApp (Lazy.force pos, [| to_pos n |])
+      then raise (Invalid_argument ("to_nat: " ^ string_of_int n))
+      else to_nat n
 
-let to_nat contrib =
-  let pos_pkg = ["Coq";"Init";"Datatypes"] in
-  let s = lazy (resolve_symbol contrib pos_pkg "S") in
-  let o = lazy (resolve_symbol contrib pos_pkg "O") in
-  let rec to_nat n =
-    if n = 0 then
-      Lazy.force o
+  let to_list =
+    let c_nil = lazy (resolve_symbol datatypes_pkg "nil") in
+    let c_cons = lazy (resolve_symbol datatypes_pkg "cons") in
+    fun typ ->
+      let the_nil = Term.mkApp (Lazy.force c_nil, [| typ |]) in
+      let rec to_list (ls : Term.constr list) : Term.constr =
+	match ls with
+	  [] -> the_nil
+	| l :: ls ->
+	  Term.mkApp (Lazy.force c_cons, [| typ ; l ; to_list ls |])
+      in to_list
+
+  type 'a pmap =
+  | PM_Empty
+  | PM_Branch of 'a pmap * 'a option * 'a pmap
+
+  let rec pmap_add k v m =
+    if k = 1 then
+      match m with
+	PM_Empty -> PM_Branch (PM_Empty, Some v, PM_Empty)
+      | PM_Branch(l,_,r) -> PM_Branch (l, Some v, r)
     else
-      Term.mkApp (Lazy.force s, [| to_nat (n - 1) |])
-  in
-  fun n ->
-    if n < 0
-    then raise (Invalid_argument ("to_nat: " ^ string_of_int n))
-    else to_nat n
+      if k mod 2 = 0 then
+	match m with
+	  PM_Empty -> PM_Branch (pmap_add (k / 2) v PM_Empty, None, PM_Empty)
+	| PM_Branch (l,d,r) -> PM_Branch (pmap_add (k / 2) v l, d, r)
+      else
+	match m with
+	  PM_Empty -> PM_Branch (PM_Empty, None, pmap_add (k / 2) v PM_Empty)
+	| PM_Branch (l,d,r) -> PM_Branch (l, d, pmap_add (k / 2) v r)
 
-let to_list contrib =
-  let list_pkg = ["Coq";"Init";"Datatypes"] in
-  let c_nil = lazy (resolve_symbol contrib list_pkg "nil") in
-  let c_cons = lazy (resolve_symbol contrib list_pkg "cons") in
-  fun typ ->
-    let the_nil = Term.mkApp (Lazy.force c_nil, [| typ |]) in
-    let rec to_list (ls : Term.constr list) : Term.constr =
+  let to_posmap (mkEmpty : 'b)
+      (mkBranch : 'b -> 'c option -> 'b -> 'b)
+      (get : 'a -> 'c option) =
+    let rec to_pm i ls acc =
       match ls with
-	[] -> the_nil
+	[] -> acc
       | l :: ls ->
-	Term.mkApp (Lazy.force c_cons, [| typ ; l ; to_list ls |])
-    in to_list
+	to_pm (1 + i) ls
+	  (match get l with
+	    None ->  acc
+	  | Some d -> pmap_add i d acc)
+    in
+    let rec convert pm =
+      match pm with
+	PM_Empty -> mkEmpty
+      | PM_Branch (l,d,r) ->
+	mkBranch (convert l) d (convert r)
+    in
+    fun ls ->
+      let pm = to_pm 1 ls PM_Empty in
+      convert pm
 
-(** TODO: It is probably easier to do a list and then build
- ** and then use gallina to build the actual pmap object
- **)
-(*
-type 'a pmap =
-| PM_Empty
-| PM_Branch of 'a pmap * 'a option * 'a pmap
-
-let rec pmap_add k v m =
-  if k = 1 then
-    match m with
-      PM_Empty -> PM_Branch (PM_Empty, Some v, PM_Empty)
-    | PM_Branch(l,_,r) -> PM_Branch (l, v, r)
-  else
-    if k mod 2 = 0 then
-      match m with
-	PM_Empty -> PM_Branch (pmap_add (k / 2) v PM_Empty, None, PM_Empty)
-      | PM_Branch (l,d,r) -> PM_Branch (pmap_add (k / 2) v l, d, r)
-    else
-      match m with
-	PM_Empty -> PM_Branch (PM_Empty, None, pmap_add (k / 2) v PM_Empty)
-      | PM_Branch (l,d,r) -> PM_Branch (l, d, pmap_add (k / 2) v r)
-
-let to_posmap contrib =
-  let pm_pkg = ["ExtLib";"Data";"Map";"FMapPositive"] in
-  let ctor_empty =
-*)
+end
 
 
 let rec app_long f acc =
